specParNoCtxtSwitch/NonSpecPureStep.v
@@ -1,9 +1,8 @@
-Require Import Spec. 
+Require Import Spec.   
 Require Import NonSpec. 
 Require Import AST.
 Require Import Coq.Sets.Ensembles.   
 Require Import sets. 
-Require Import CpdtTactics. 
 Require Import SfLib. 
 
 Ltac applyHyp :=
@@ -17,13 +16,15 @@ Fixpoint alphaConvert t x y :=
       |punit => punit
       |ppair e1 e2 => ppair (alphaConvert e1 x y) (alphaConvert e2 x y)
       |pvar z => if beq_nat x z then pvar y else t
-      |plambda z e => if beq_nat x z then plambda y (alphaConvert e x y) else plambda z (alphaConvert e x y)
+      |plambda z e => if beq_nat x z then plambda y (alphaConvert e x y) 
+                      else plambda z (alphaConvert e x y)
       |papp e1 e2 => papp (alphaConvert e1 x y) (alphaConvert e2 x y)
       |pret e => pret (alphaConvert e x y)
       |pbind e1 e2 => pbind (alphaConvert e1 x y) (alphaConvert e2 x y)
       |pfork e => pfork (alphaConvert e x y)
       |pnew => pnew
-      |pput z e => if beq_nat x y then pput y (alphaConvert e x y) else pput z (alphaConvert e x y)
+      |pput z e => if beq_nat x y then pput y (alphaConvert e x y) 
+                   else pput z (alphaConvert e x y)
       |pget z => if beq_nat x y then pget y else t
       |praise e => praise (alphaConvert e x y)
       |phandle e1 e2 => phandle (alphaConvert e1 x y) (alphaConvert e2 x y)
@@ -34,42 +35,168 @@ Fixpoint alphaConvert t x y :=
 
 Axiom alphaEqual : forall t x y t2, alphaConvert t x y = t2 -> t = t2. 
 
-Theorem termErasureDeterminsim : forall M T M1 M2,
+Theorem termErasureDeterminism : forall M T M1 M2,
                                    eraseTerm M T M1 -> eraseTerm M T M2 -> M1 = M2. 
 Proof.
-  intros. generalize dependent M2. induction H; intros; try(inversion H0; reflexivity);
+  intros. generalize dependent M2. induction H; intros; 
+                                   try(inversion H0; reflexivity);
   try(clear H; clear H0; match goal with
                            |H:eraseTerm ?T ?T' ?M |- _ => 
-                            inversion H; clear H; applyHyp; applyHyp; subst; reflexivity
+                    inversion H; clear H; applyHyp; applyHyp; subst; reflexivity
                          end); 
   try(clear H; match goal with
                 |H : eraseTerm ?T ?T' ?M |- _ =>
                  inversion H; clear H; applyHyp; subst; reflexivity
                end). 
-  {inversion H2. subst. apply IHeraseTerm1 in H5. apply IHeraseTerm2 in H6. 
-   subst. assert(pbind e1'0
-     (plambda i (pbind e2'0 (plambda j (pret (ppair (pvar i) (pvar j)))))) =
-   pbind e1'0
-     (plambda i (pbind e2'0 (plambda j0 (pret (ppair (pvar i0) (pvar j0))))))). 
-   apply alphaEqual with (x := j)(y := j0). simpl. 
+  {admit. }{admit. }
+Qed. 
 
+Theorem lastElementEq : forall (T:Type) l1 l2 (e1 e2 : T),
+                          l1 ++ [e1] = l2 ++ [e2] -> e1 = e2. 
+Proof.
+  intros. generalize dependent l2. induction l1; intros. 
+  {destruct l2. 
+   {inversion H. reflexivity. }
+   {inversion H. destruct l2; inversion H2. }
+  }
+  {destruct l2. 
+   {simpl in *. inversion H. destruct l1; inversion H2. }
+   {simpl in *. inversion H. apply IHl1 in H2. assumption. }
+  }
+Qed. 
 
 Theorem erasureDeterminism : forall t t1' t2' T, 
-                               eraseThread t T t1' -> eraseThread t T t2' -> t1' = t2'.
+                               eraseThread t T t1' -> 
+                               eraseThread t T t2' -> t1' = t2'.
 Proof.
-  intros. inversion H. 
-  {subst. inversion H0. subst. 
+  intros. induction H; inversion H0;
+  try(subst; match goal with
+               |H:eraseTerm ?M ?T ?x, H':eraseTerm ?M ?T ?y |- _ =>
+                eapply termErasureDeterminism in H;[rewrite<-H;reflexivity|auto]
+               |H:[] = [] ++ [?x] |- _ => inversion H       
+               |H:[] = ?x ++ [?y] |- _ => destruct x; inversion H
+               |H:?s1++[?x]=?s2++[?y]|-_ => apply lastElementEq in H; inversion H
+             end);
+  try(subst; eapply termErasureDeterminism in H9;[rewrite <-H9; reflexivity| auto]);
+  reflexivity. Qed. 
+  
+Theorem eraseHeapDeterminism : forall h h1 h2, 
+                                 eraseHeap h h1 -> eraseHeap h h2 ->
+                                 h1 = h2. 
+Proof.
+  intros. generalize dependent h2. induction H; intros. 
+  {inversion H0. subst. apply IHeraseHeap in H6. assumption. }
+  {inversion H0. subst. apply IHeraseHeap in H4. subst. reflexivity. }
+  {inversion H0; subst. apply IHeraseHeap in H10. assumption. }
+  {inversion H0. subst. apply IHeraseHeap in H9. subst. reflexivity. }
+  {inversion H1. subst. apply IHeraseHeap in H8. subst. 
+   eapply termErasureDeterminism in H0. rewrite <-H0. reflexivity. assumption. }
+Qed. 
 
+Require Import Coq.Program.Equality. 
+ 
+Theorem pdecomposeNotVal : forall M E e,
+                             pdecompose M E e -> ~pvalue M. 
+Proof.
+  intros. inversion H; subst; intros c; inversion c. Qed. 
 
-Theorem NonSpecPureStep : forall h h' sh sh' tid s1 s2 M tid' M' t t', 
-                            multistep h tEmptySet (tSingleton (tid, s1, s2, M)) h' 
-                                      tEmptySet (tSingleton(tid', s1, s2, M')) ->
-                            eraseThread (tid, s1, s2, M) tEmptySet (pSingleton t) ->
-                            eraseThread (tid', s1, s2, M') tEmptySet (pSingleton t') ->
+Theorem eraseValue : forall M T e, value M -> eraseTerm M T e -> pvalue e. 
+Proof.
+  intros. inversion H0; subst; try inversion H; try constructor. Qed. 
+
+Theorem erasureDecompose : forall t T pt E e,
+                             eraseTerm t T pt -> decompose t E e ->
+                             exists E' e', eraseTerm e T e' /\ pdecompose pt E' e'. 
+Proof.
+  intros. generalize dependent pt. induction H0. 
+  {intros. inversion H2; subst. apply IHdecompose in H5. inversion H5. 
+   inversion H3. inversion H4. econstructor. exists x0. split. 
+   assumption. econstructor. apply pdecomposeNotVal in H7. assumption. 
+   eassumption. }
+  {intros. inversion H0; subst. econstructor. econstructor. split. 
+   eassumption. eapply bindCtxtValue. eapply eraseValue in H. eassumption. 
+   eassumption. }
+  {intros. inversion H2; subst. apply IHdecompose in H5. inversion H5. 
+   inversion H3. inversion H4. econstructor. exists x0. split. assumption. 
+   econstructor. apply pdecomposeNotVal in H9. assumption. eassumption. }
+  {intros. inversion H0; subst. econstructor. econstructor. split. 
+   eassumption. eapply bindCtxtValue. eapply eraseValue in H. eassumption. 
+   eassumption. }
+  {intros. inversion H2; subst. apply IHdecompose in H5. inversion H5. 
+   inversion H3. inversion H4. econstructor. econstructor. split. eassumption. 
+   econstructor. apply pdecomposeNotVal in H7. assumption. eassumption. }
+  {intros. inversion H0; subst. econstructor. econstructor. split. eassumption. 
+   eapply handleCtxtValue. eapply eraseValue in H. eassumption. eassumption. }
+Qed. 
+
+Theorem erasureDecompose' : forall t T pt E e e',
+                             eraseTerm t T pt -> decompose t E e ->
+                             eraseTerm e T e' -> 
+                             exists E', pdecompose pt E' e'. 
+Proof.
+  intros. generalize dependent pt. generalize dependent e'. induction H0. 
+  {intros. inversion H1; 
+   try(subst; inversion H2; subst; inversion H3; subst; eapply IHdecompose in H2; 
+    inversion H2; [econstructor; econstructor;[apply pdecomposeNotVal in H4| 
+    eassumption]; eassumption |assumption]). }
+  {intros; apply termErasureDeterminism with (M1:=pt)in H1; [subst; econstructor; 
+   inversion H0; subst; econstructor; eapply eraseValue in H; [eassumption|
+   eassumption]|assumption]. }
+  {intros. inversion H1; 
+    try(subst; inversion H2; subst; inversion H3; subst; eapply IHdecompose in H2; 
+    inversion H2; [econstructor; econstructor;[apply pdecomposeNotVal in H4| 
+    eassumption]; eassumption |assumption]). }
+ {intros; apply termErasureDeterminism with (M1:=pt)in H1; [subst; econstructor; 
+   inversion H0; subst; econstructor; eapply eraseValue in H; [eassumption|
+   eassumption]|assumption]. }   
+ {intros. inversion H1; 
+    try(subst; inversion H2; subst; inversion H3; subst; eapply IHdecompose in H2; 
+    inversion H2; [econstructor; econstructor;[apply pdecomposeNotVal in H4| 
+    eassumption]; eassumption |assumption]). }
+ {intros; apply termErasureDeterminism with (M1:=pt)in H1; [subst; econstructor; 
+   inversion H0; subst; econstructor; eapply eraseValue in H; [eassumption|
+   eassumption]|assumption]. }  
+Qed. 
+
+Ltac copy H := 
+  match type of H with
+      |?X => assert(X) by apply H
+  end. 
+
+Theorem eraseHole : forall E E' t (e1 e2:term) (e1' e2':pterm) T,
+                      decompose t E e1 ->
+                      eraseTerm t T (E' e1') ->
+                      eraseTerm e2 T e2' ->
+                      eraseTerm (E e2) T (E' e2').
+Proof.
+  intros. remember (E' e1'). induction H0; try(solve[inversion H]). 
+  {
+
+Require Import Coq.Sets.Powerset_facts. 
+Theorem NonSpecPureStep : forall h h' sh sh' t t' pt pt' tid tid' s1 s2 M M',
+                            t = tSingleton (tid,s1,s2,M) -> 
+                            t' = tSingleton(tid',s1,s2,M') ->
+                            multistep h tEmptySet t h' tEmptySet t' ->
+                            eraseTerm M tEmptySet pt ->
+                            eraseTerm M' tEmptySet pt' ->
                             eraseHeap h sh -> eraseHeap h' sh' ->
-                            pmultistep sh (Empty_set pterm) (pSingleton t) sh' (Empty_set pterm) (pSingleton t'). 
+                            pmultistep sh (Empty_set pterm)(pSingleton pt) sh'
+                                       (Empty_set pterm) (pSingleton pt').
 Proof.
-  intros. remember (tSingleton(tid, s1, s2, M)). remember (tSingleton (tid', s1, s2, M')).  induction H. 
-  {subst. inversion Heqe0. apply SingletonEq in H4. inversion H4. subst. 
-   
+  intros. generalize dependent tid'. generalize dependent M'. 
+  generalize dependent pt. generalize dependent M. induction H1. 
+  {intros. subst. apply SingletonEq in H0. inversion H0. subst. 
+   eapply termErasureDeterminism in H2. eapply eraseHeapDeterminism in H4. 
+   rewrite <- H2. rewrite <- H4. econstructor. assumption. assumption. }
+  {intros. inversion H1; subst. 
+   {symmetry in H. apply disjointUnionEqSingleton with(e2:=(tid,s1,s2,M))in H0. 
+    inversion H0. copy H9. apply decomposeEq in H9. subst t.  copy H6. 
+    eapply erasureDecompose with (e:=bind(ret M0) N)in H6. inversion H6. 
+    inversion H11. inversion H12. inversion H13. inversion H17. 
+    eapply pSingletonMultistep. econstructor. 
+    intros c. inversion c. apply PBind. subst x0. subst e1'. eassumption. 
+    unfold pUnion. unfold pSingleton. rewrite Union_commutative. rewrite union_empty. 
+    eapply IHmultistep. assumption. assumption. subst. rewrite <- union_empty. 
+    rewrite Union_commutative. unfold tUnion. inversion H3. subst. reflexivity. 
+    subst. 
 
